src/PredCrash.v
@@ -9,41 +9,43 @@ Require Export AsyncDisk.
 
 Set Implicit Arguments.
 
-Definition ptsto_subset {AT AEQ} (a : AT) (vs : valuset) : @pred AT AEQ valuset :=
+Definition ptsto_subset {AT AEQ V} (a : AT) (vs : V * list V) : @pred AT AEQ (V * list V) :=
   (exists old, a |-> (fst vs, old) * [[ incl old (snd vs) ]])%pred.
 
-Notation "a |=> v" := (a |-> ((v, nil) : valuset))%pred (at level 35) : pred_scope.
-Notation "a |~> v" := (exists old, a |-> ((v, old) : valuset))%pred (at level 35) : pred_scope.
+Notation "a |=> v" := (a |-> (v, nil))%pred (at level 35) : pred_scope.
+Notation "a |~> v" := (exists old, a |-> (v, old))%pred (at level 35) : pred_scope.
 Notation "a |+> v" := (ptsto_subset a v) (at level 35) : pred_scope.
 Notation "a |+>?" := (exists v, a |+> v)%pred (at level 35) : pred_scope.
 
-Definition rawpred := @pred addr addr_eq_dec valuset.
+Definition rawpred V := @pred addr addr_eq_dec (V * list V).
 
-Definition possible_crash (m m' : rawdisk) : Prop :=
+Definition possible_crash {AT AEQ V} (m m' : @mem AT AEQ (V * list V)) : Prop :=
   forall a,
   (m a = None /\ m' a = None) \/
   (exists vs v', m a = Some vs /\ m' a = Some (v', nil) /\ In v' (vsmerge vs)).
 
 (* if [p] was true before a crash, then [crash_xform p] is true after a crash *)
-Definition crash_xform (p : rawpred) : rawpred :=
+Definition crash_xform {AT AEQ V} (p : @pred AT AEQ (V * list V)) :=
   fun m => exists m', p m' /\ possible_crash m' m.
 
 (* if [p] was true before a sync, then [sync_xform p] is true after a sync *)
-Definition sync_xform (p : rawpred) : rawpred :=
+Definition sync_xform {AT AEQ V} (p : @pred AT AEQ (V * list V)) :=
   fun m => exists m', p m' /\ m = sync_mem m'.
 
 
 (* Specialized relations for [@pred valuset], to deal with async IO *)
 
-Theorem crash_xform_apply : forall (p : rawpred) (m m' : rawdisk), possible_crash m m'
+Theorem crash_xform_apply : forall {AT AEQ V} (p : @pred AT AEQ (V * list V))  m m',
+    possible_crash m m'
   -> p m
   -> crash_xform p m'.
 Proof.
   unfold crash_xform; eauto.
 Qed.
 
-Theorem possible_crash_mem_union : forall (ma mb m' : rawdisk), possible_crash (mem_union ma mb) m'
-  -> @mem_disjoint _ addr_eq_dec _ ma mb
+Theorem possible_crash_mem_union : forall AT AEQ V (ma mb m' : @mem AT AEQ (V * list V)),
+    possible_crash (mem_union ma mb) m'
+  -> mem_disjoint ma mb
   -> exists ma' mb', m' = mem_union ma' mb' /\ mem_disjoint ma' mb' /\
                      possible_crash ma ma' /\ possible_crash mb mb'.
 Proof.
@@ -80,11 +82,11 @@ Proof.
     congruence.
 Qed.
 
-Theorem possible_crash_disjoint : forall (ma mb ma' mb' : rawdisk),
-  @mem_disjoint _ addr_eq_dec _ ma' mb'
+Theorem possible_crash_disjoint : forall AT AEQ V (ma mb ma' mb' : @mem AT AEQ (V * list V)),
+  mem_disjoint  ma' mb'
   -> possible_crash ma ma'
   -> possible_crash mb mb'
-  -> @mem_disjoint _ addr_eq_dec _ ma mb.
+  -> mem_disjoint ma mb.
 Proof.
   unfold mem_disjoint, possible_crash; intros.
   intro Hnot.
@@ -95,7 +97,8 @@ Proof.
   do 3 eexists; eauto.
 Qed.
 
-Theorem possible_crash_union : forall (ma mb ma' mb' : rawdisk), possible_crash ma ma'
+Theorem possible_crash_union : forall AT AEQ V (ma mb ma' mb' : @mem AT AEQ (V * list V)),
+    possible_crash ma ma'
   -> possible_crash mb mb'
   -> possible_crash (mem_union ma mb) (mem_union ma' mb').
 Proof.
@@ -115,7 +118,7 @@ Proof.
     right. do 2 eexists. intuition.
 Qed.
 
-Theorem possible_crash_trans : forall (ma mb mc : rawdisk),
+Theorem possible_crash_trans : forall AT AEQ V (ma mb mc : @mem AT AEQ (V * list V)),
   possible_crash ma mb ->
   possible_crash mb mc ->
   possible_crash ma mc.
@@ -133,7 +136,7 @@ Proof.
 Qed.
 
 
-Lemma possible_crash_notindomain : forall AEQ (m m' : @mem _ AEQ _) a,
+Lemma possible_crash_notindomain : forall AT AEQ V (m m' : @mem AT AEQ (V * list V)) a,
   possible_crash m m' ->
   notindomain a m ->
   notindomain a m'.
@@ -143,19 +146,19 @@ Proof.
 Qed.
 
 
-Lemma possible_crash_upd : forall m m' a v vs,
+Lemma possible_crash_upd : forall AT AEQ V (m m' : @mem AT AEQ (V * list V)) a v vs,
   possible_crash m m' ->
   In v (vsmerge vs) ->
   possible_crash (upd m a vs) (upd m' a (v, nil)).
 Proof.
   unfold possible_crash; intuition.
-  destruct (addr_eq_dec a a0); subst.
+  destruct (AEQ a a0); subst.
   repeat rewrite upd_eq; auto.
   specialize (H a0); intuition; right; eexists; eauto.
   repeat rewrite upd_ne; auto.
 Qed.
 
-Lemma possible_crash_updSome : forall m m' a v vs,
+Lemma possible_crash_updSome : forall AT AEQ V (m m' : @mem AT AEQ (V * list V)) a v vs,
   possible_crash m m' ->
   In v (vsmerge vs) ->
   possible_crash (updSome m a vs) (updSome m' a (v, nil)).
@@ -166,15 +169,15 @@ Proof.
   - repeat rewrite updSome_none by eauto.
     intuition.
 
-  - destruct (addr_eq_dec a a0); subst.
+  - destruct (AEQ a a0); subst.
     + repeat erewrite updSome_eq by eauto. right. eauto.
     + repeat rewrite updSome_ne by eauto. eauto.
 Qed.
 
-Definition synced_mem (m : rawdisk) :=
+Definition synced_mem {AT AEQ V} (m : @mem AT AEQ (V * list V)) :=
   forall a, m a = None \/ exists v, m a = Some (v, nil).
 
-Lemma synced_mem_snd_nil : forall m a vs,
+Lemma synced_mem_snd_nil : forall AT AEQ V (m : @mem AT AEQ (V * list V)) a vs,
   synced_mem m ->
   m a = Some vs ->
   snd vs = nil.
@@ -185,7 +188,7 @@ Proof.
   rewrite H in H0; inversion H0; auto.
 Qed.
 
-Theorem possible_crash_synced : forall m m',
+Theorem possible_crash_synced : forall AT AEQ V (m m' : @mem AT AEQ (V * list V)),
   possible_crash m m' ->
   synced_mem m'.
 Proof.
@@ -195,7 +198,7 @@ Proof.
   eexists; eauto.
 Qed.
 
-Theorem possible_crash_refl : forall m,
+Theorem possible_crash_refl : forall AT AEQ V (m : @mem AT AEQ (V * list V)),
   synced_mem m ->
   possible_crash m m.
 Proof.
@@ -206,7 +209,7 @@ Proof.
 Qed.
 
 
-Lemma possible_crash_emp_l : forall (m m' : @mem _ addr_eq_dec _),
+Lemma possible_crash_emp_l : forall AT AEQ V (m m' : @mem AT AEQ (V * list V)),
   possible_crash m m' ->
   emp m' ->
   emp m.
@@ -216,7 +219,7 @@ Proof.
   congruence.
 Qed.
 
-Lemma possible_crash_emp_r : forall (m m' : @mem _ addr_eq_dec _),
+Lemma possible_crash_emp_r : forall AT AEQ V (m m': @mem AT AEQ (V * list V)),
   possible_crash m m' ->
   emp m ->
   emp m'.
@@ -226,7 +229,7 @@ Proof.
   congruence.
 Qed.
 
-Lemma possible_crash_ptsto_upd_incl' : forall m m' a vs vs',
+Lemma possible_crash_ptsto_upd_incl' : forall AT AEQ V (m m': @mem AT AEQ (V * list V)) a vs vs',
   m a = Some vs ->
   possible_crash m m' ->
   incl (vsmerge vs) (vsmerge vs') ->
@@ -234,22 +237,22 @@ Lemma possible_crash_ptsto_upd_incl' : forall m m' a vs vs',
 Proof.
   unfold possible_crash, vsmerge; simpl; intros.
   destruct vs, vs'; simpl in *.
-  destruct (addr_eq_dec a0 a); subst.
+  destruct (AEQ a0 a); subst.
 
   - specialize (H0 a); intuition.
     left; congruence.
     right; erewrite upd_eq by eauto; repeat deex; destruct vs; simpl in *.
     rewrite H in H2; inversion H2; subst.
-    exists (t0, l0); exists t1; intuition.
+    exists (v0, l0); exists v1; intuition.
     rewrite H in H2; inversion H2; subst.
-    exists (t0, l0); exists v'; intuition.
+    exists (v0, l0); exists v'; intuition.
 
   - rewrite upd_ne by auto.
     specialize (H0 a0); intuition.
 Qed.
 
 
-Lemma possible_crash_ptsto_upd_incl : forall F m m' a vs vs',
+Lemma possible_crash_ptsto_upd_incl : forall AT AEQ V F (m m': @mem AT AEQ (V * list V)) a vs vs',
   (F * a |-> vs)%pred m ->
   possible_crash m m' ->
   incl (vsmerge vs) (vsmerge vs') ->
@@ -260,25 +263,25 @@ Proof.
   eapply ptsto_valid'; eauto.
 Qed.
 
-Lemma possible_crash_upd_incl : forall m m' a v v0,
+Lemma possible_crash_upd_incl : forall AT AEQ V (m m' : @mem AT AEQ (V * list V)) a v v0,
   possible_crash (upd m a v) m' ->
   m a = Some v0 ->
   incl (vsmerge v) (vsmerge v0) ->
   possible_crash m m'.
 Proof.
   unfold possible_crash, vsmerge; intuition.
-  destruct (addr_eq_dec a a0); subst; simpl in *.
-  - specialize (H a0); intuition; right;
+  destruct (AEQ a a1); subst; simpl in *.
+  - specialize (H a1); intuition; right;
     erewrite upd_eq in * by eauto; try congruence.
     repeat deex.
     destruct vs, v0; inversion H2; subst; simpl in *.
-    exists (t0, l0), t; intuition.
+    exists (v0, l0), v; intuition.
     destruct vs, v0; inversion H2; subst; simpl in *.
-    exists (t0, l0), v'; intuition.
-  - specialize (H a0); intuition; rewrite upd_ne in *; auto.
+    exists (v0, l0), v'; intuition.
+  - specialize (H a1); intuition; rewrite upd_ne in *; auto.
 Qed.
 
-Lemma possible_crash_upd_nil : forall m m' a v0,
+Lemma possible_crash_upd_nil : forall AT AEQ V (m m': @mem AT AEQ (V * list V)) a v0,
   possible_crash (upd m a (fst v0, nil)) m' ->
   m a = Some v0 ->
   possible_crash m m'.
@@ -290,7 +293,7 @@ Proof.
 Qed.
 
 
-Lemma possible_crash_ptsto_upd_postfix : forall F m m' a v vs vs',
+Lemma possible_crash_ptsto_upd_postfix : forall AT AEQ V F (m m' : @mem AT AEQ (V * list V)) a v vs vs',
   (F * a |-> (v, vs))%pred m ->
   possible_crash m m' ->
   postfix vs vs' ->
@@ -303,7 +306,7 @@ Proof.
   eapply in_skipn_in; eauto.
 Qed.
 
-Lemma possible_crash_sel_exis : forall m m' a vs,
+Lemma possible_crash_sel_exis : forall AT AEQ V (m m' : @mem AT AEQ (V * list V)) a vs,
   possible_crash m m' ->
   m a = Some vs ->
   exists v, m' a = Some (v, nil) /\ In v (vsmerge vs).
@@ -315,7 +318,7 @@ Proof.
 Qed.
 
 
-Theorem crash_xform_sep_star_dist : forall (p q : rawpred),
+Theorem crash_xform_sep_star_dist : forall AT AEQ V (p q: @pred AT AEQ (V * list V)),
   crash_xform (p * q) <=p=> crash_xform p * crash_xform q.
 Proof.
   unfold_sep_star; unfold crash_xform, piff, pimpl; split; intros; repeat deex.
@@ -327,14 +330,14 @@ Proof.
     apply possible_crash_union; eauto.
 Qed.
 
-Theorem crash_xform_or_dist : forall (p q : rawpred),
+Theorem crash_xform_or_dist : forall AT AEQ V (p q: @pred AT AEQ (V * list V)),
   crash_xform (p \/ q) <=p=> crash_xform p \/ crash_xform q.
 Proof.
   firstorder.
 Qed.
 
-Theorem crash_xform_lift_empty : forall (P : Prop),
-  @crash_xform [[ P ]] <=p=> [[ P ]].
+Theorem crash_xform_lift_empty : forall AT AEQ V (P : Prop),
+  @crash_xform AT AEQ V [[ P ]] <=p=> [[ P ]].
 Proof.
   unfold crash_xform, lift_empty, possible_crash; intros; split;
     intros m H; repeat deex.
@@ -343,7 +346,8 @@ Proof.
   eexists; intuition.
 Qed.
 
-Theorem crash_xform_sep_star_apply : forall (p q : rawpred) (m m' : mem), possible_crash m m'
+Theorem crash_xform_sep_star_apply : forall AT AEQ V (p q: @pred AT AEQ (V * list V)) (m m' : mem),
+    possible_crash m m'
   -> (p * q)%pred m
   -> (crash_xform p * crash_xform q)%pred m'.
 Proof.
@@ -352,22 +356,22 @@ Proof.
   do 2 eexists; repeat split; auto; unfold crash_xform; eexists; split; eauto.
 Qed.
 
-Theorem crash_xform_exists_comm : forall T (p : T -> rawpred),
+Theorem crash_xform_exists_comm : forall T AT AEQ V (p : T -> @pred AT AEQ (V * list V)),
   crash_xform (exists x, p x) <=p=> exists x, crash_xform (p x).
 Proof.
   split; unfold crash_xform, exis, pimpl; intros;
   repeat deex; repeat eexists; intuition eauto.
 Qed.
 
-Theorem crash_xform_forall_comm : forall T (p : T -> rawpred),
+Theorem crash_xform_forall_comm : forall T AT AEQ V (p : T -> @pred AT AEQ (V * list V)),
   crash_xform (foral x, p x) =p=> foral x, crash_xform (p x).
 Proof.
   unfold crash_xform, foral_, pimpl; intros.
   repeat deex; repeat eexists; intuition eauto.
 Qed.
 
-Theorem crash_xform_ptsto: forall a v,
-  crash_xform (a |-> v) =p=> exists v', [[ In v' (vsmerge v) ]] * a |=> v'.
+Theorem crash_xform_ptsto: forall A AEQ V (a: A) (v: V * list V),
+  (crash_xform (AEQ:=AEQ)) (a |-> v) =p=> exists v', [[ In v' (vsmerge v) ]] * a |=> v'.
 Proof.
   unfold crash_xform, possible_crash, ptsto, pimpl; intros.
   repeat deex; destruct (H1 a).
@@ -385,28 +389,28 @@ Proof.
   congruence.
 Qed.
 
-Theorem crash_xform_ptsto_r: forall a v vs,
+Theorem crash_xform_ptsto_r: forall A AEQ V a v vs,
   In v (vsmerge vs) ->
-  a |=> v =p=> crash_xform (a |-> vs).
+  a |=> v =p=> @crash_xform A AEQ V (a |-> vs).
 Proof.
   unfold crash_xform, possible_crash, ptsto, pimpl; intros.
   exists (insert empty_mem a vs).
   intuition.
   rewrite insert_eq; eauto.
   rewrite insert_ne; eauto.
-  destruct (eq_nat_dec a a0); subst.
+  destruct (AEQ a a0); subst.
   - right. rewrite insert_eq; auto. exists vs. exists v. intuition.
   - left. rewrite insert_ne; auto.
 Qed.
 
 
-Theorem crash_xform_ptsto_exis : forall a,
-  crash_xform ( a |->? ) =p=> a |->?.
+Theorem crash_xform_ptsto_exis : forall A AEQ V a,
+  @crash_xform A AEQ V ( a |->? ) =p=> a |->?.
 Proof.
   intros.
   rewrite crash_xform_exists_comm.
   apply pimpl_exists_l; intro.
-  rewrite crash_xform_ptsto.
+  setoid_rewrite crash_xform_ptsto.
   apply pimpl_exists_l; intro.
   apply pimpl_exists_r.
   exists (x0, nil).
@@ -414,8 +418,8 @@ Proof.
   apply sep_star_lift_l; intros; auto.
 Qed.
 
-Theorem crash_xform_ptsto_subset : forall a v,
-  crash_xform (a |+> v) =p=> exists v', [[ In v' (vsmerge v) ]] * a |=> v'.
+Theorem crash_xform_ptsto_subset : forall A AEQ V a v,
+  @crash_xform A AEQ V (a |+> v) =p=> exists v', [[ In v' (vsmerge v) ]] * a |=> v'.
 Proof.
   unfold ptsto_subset; intros.
   rewrite crash_xform_exists_comm.
@@ -433,9 +437,9 @@ Proof.
   cbn in *; intuition.
 Qed.
 
-Theorem crash_xform_ptsto_subset_r: forall a v vs,
+Theorem crash_xform_ptsto_subset_r: forall A AEQ V a v vs,
   In v (vsmerge vs) ->
-  a |=> v =p=> crash_xform (a |+> vs).
+  a |=> v =p=> @crash_xform A AEQ V (a |+> vs).
 Proof.
   unfold ptsto_subset; intros.
   rewrite crash_xform_exists_comm.
@@ -450,46 +454,48 @@ Proof.
 Qed.
 
 
-Theorem crash_xform_pimpl : forall (p q : rawpred), p =p=>q
+Theorem crash_xform_pimpl : forall {AT AEQ V} (p q: @pred AT AEQ (V * list V)), p =p=>q
   -> crash_xform p =p=> crash_xform q.
 Proof.
   firstorder.
 Qed.
 
+
 Instance crash_xform_pimpl_proper:
-  Proper (pimpl ==> pimpl) crash_xform.
+  forall AT AEQ V, Proper (pimpl ==> pimpl) (@crash_xform AT AEQ V).
 Proof.
   firstorder.
 Qed.
 
 Instance crash_xform_flip_pimpl_proper:
-  Proper (Basics.flip pimpl ==> Basics.flip pimpl) crash_xform.
+  forall AT AEQ V, Proper (Basics.flip pimpl ==> Basics.flip pimpl) (@crash_xform AT AEQ V).
 Proof.
   firstorder.
 Qed.
 
 Instance crash_xform_piff_proper:
-  Proper (piff ==> piff) crash_xform.
+  forall AT AEQ V, Proper (piff ==> piff) (@crash_xform AT AEQ V).
 Proof.
   firstorder.
 Qed.
 
+
 Theorem crash_invariant_emp:
-  crash_xform emp =p=> emp.
+  forall AT AEQ V, @crash_xform AT AEQ V emp =p=> emp.
 Proof.
   unfold crash_xform, possible_crash, emp, pimpl; repeat deex; intuition; repeat deex.
   destruct (H1 a); [ intuition | repeat deex; congruence ].
 Qed.
 
 Theorem crash_invariant_emp_r:
-  emp =p=> crash_xform emp.
+  forall AT AEQ V, emp =p=> @crash_xform AT AEQ V emp.
 Proof.
   unfold crash_xform, possible_crash, emp, pimpl. intros.
   exists empty_mem. intuition.
 Qed.
 
-Theorem crash_invariant_ptsto: forall a v,
-  crash_xform (a |=> v) =p=> a |=> v.
+Theorem crash_invariant_ptsto: forall AT AEQ V a v,
+  @crash_xform AT AEQ V (a |=> v) =p=> a |=> v.
 Proof.
   unfold crash_xform, pimpl, possible_crash, ptsto; intros.
   deex; intuition eauto.
@@ -505,7 +511,7 @@ Proof.
 Qed.
 
 Lemma ptsto_synced_valid:
-  forall a v (F : rawpred) m,
+  forall AT AEQ V a v (F : @pred AT AEQ (V * list V)) m,
   (a |=> v * F)%pred m
   -> m a = Some (v, nil).
 Proof.
@@ -514,7 +520,7 @@ Proof.
 Qed.
 
 Lemma ptsto_cur_valid:
-  forall a v (F : rawpred) m,
+   forall AT AEQ V a v (F : @pred AT AEQ (V * list V)) m,
   (a |~> v * F)%pred m
   -> exists l, m a = Some (v, l).
 Proof.
@@ -526,7 +532,7 @@ Proof.
   apply mem_union_addr; eauto.
 Qed.
 
-Lemma crash_xform_diskIs: forall m,
+Lemma crash_xform_diskIs: forall AT AEQ V (m: @mem AT AEQ (V * list V)),
   crash_xform (diskIs m) =p=> exists m', [[ possible_crash m m' ]] * diskIs m'.
 Proof.
   unfold crash_xform, pimpl, diskIs.
@@ -542,7 +548,7 @@ Proof.
   unfold lift_empty; intuition.
 Qed.
 
-Lemma crash_xform_diskIs_r: forall m m',
+Lemma crash_xform_diskIs_r:  forall AT AEQ V (m m': @mem AT AEQ (V * list V)),
   possible_crash m m' ->
   diskIs m' =p=> crash_xform (diskIs m).
 Proof.
@@ -550,7 +556,7 @@ Proof.
   intros; subst; firstorder.
 Qed.
 
-Lemma crash_xform_diskIs_piff: forall m,
+Lemma crash_xform_diskIs_piff:  forall AT AEQ V (m: @mem AT AEQ (V * list V)),
   crash_xform (diskIs m) <=p=> exists m', [[ possible_crash m m' ]] * diskIs m'.
 Proof.
   split.
@@ -561,13 +567,13 @@ Proof.
   apply crash_xform_diskIs_r; auto.
 Qed.
 
-Lemma possible_crash_mem_except : forall m1 m2 a,
+Lemma possible_crash_mem_except :  forall AT AEQ V (m1 m2: @mem AT AEQ (V * list V)) a,
   possible_crash m1 m2 ->
   possible_crash (mem_except m1 a) (mem_except m2 a).
 Proof.
   unfold possible_crash, mem_except; intuition.
   specialize (H a0).
-  destruct (addr_eq_dec a0 a); intuition.
+  destruct (AEQ a0 a); intuition.
 Qed.
 
 Lemma mem_except_upd : forall AT AEQ V (m : @mem AT AEQ V) a v,
@@ -578,7 +584,7 @@ Proof.
   destruct (AEQ x a); intuition.
 Qed.
 
-Lemma possible_crash_upd_mem_except : forall m1 m2 a v,
+Lemma possible_crash_upd_mem_except :  forall AT AEQ V (m1 m2: @mem AT AEQ (V * list V)) a v,
   possible_crash m1 (upd m2 a v) ->
   possible_crash (mem_except m1 a) (mem_except m2 a).
 Proof.
@@ -589,7 +595,7 @@ Proof.
 Qed.
 
 
-Lemma possible_crash_eq : forall a b c,
+Lemma possible_crash_eq : forall AT AEQ V (a b c: @mem AT AEQ (V * list V)),
   possible_crash a b ->
   possible_crash b c ->
   b = c.
@@ -605,7 +611,7 @@ Proof.
   intuition; subst; congruence.
 Qed.
 
-Lemma crash_xform_diskIs_trans : forall d x d',
+Lemma crash_xform_diskIs_trans :  forall AT AEQ V (d d' x : @mem AT AEQ (V * list V)),
   crash_xform (diskIs d) x ->
   crash_xform (diskIs x) d' ->
   crash_xform (diskIs x) =p=> crash_xform (diskIs d).
@@ -627,7 +633,7 @@ Proof.
 Qed.
 
 
-Lemma crash_xform_diskIs_eq : forall F a b,
+Lemma crash_xform_diskIs_eq :  forall AT AEQ V (a b: @mem AT AEQ (V * list V)) F,
   crash_xform F a ->
   crash_xform (diskIs a) b ->
   a = b.
@@ -648,7 +654,7 @@ Proof.
 Qed.
 
 
-Lemma crash_xform_diskIs_pred : forall (F : pred) m,
+Lemma crash_xform_diskIs_pred :  forall AT AEQ V (m: @mem AT AEQ (V * list V)) (F: pred),
   F m -> crash_xform (diskIs m) =p=> crash_xform F.
 Proof.
   unfold crash_xform, diskIs.
@@ -657,8 +663,8 @@ Proof.
   eexists; eauto.
 Qed.
 
-Lemma crash_xform_ptsto_or : forall (a : addr) (vs : valuset),
-  crash_xform (a |-> vs) <=p=> crash_xform (a |-> vs \/ a |=> (fst vs)).
+Lemma crash_xform_ptsto_or : forall AT AEQ V a vs,
+  @crash_xform AT AEQ V (a |-> vs) <=p=> crash_xform (a |-> vs \/ a |=> (fst vs)).
 Proof.
   split.
   rewrite crash_xform_or_dist.
@@ -674,8 +680,8 @@ Proof.
 Qed.
 
 
-Lemma crash_xform_ptsto_vsmerge :  forall (a : addr) (vs : valuset) (v : tagged_block),
-  crash_xform (a |-> (v, vsmerge vs)) <=p=> crash_xform (a |-> vs \/ a |-> (v, vsmerge vs)).
+Lemma crash_xform_ptsto_vsmerge :  forall AT AEQ V a vs v,
+  @crash_xform AT AEQ V (a |-> (v, vsmerge vs)) <=p=> crash_xform (a |-> vs \/ a |-> (v, vsmerge vs)).
 Proof.
   split; rewrite crash_xform_or_dist.
   apply pimpl_or_r; right; auto.
@@ -689,7 +695,7 @@ Proof.
 Qed.
 
 
-Theorem crash_xform_idem_l : forall (p : rawpred), 
+Theorem crash_xform_idem_l : forall AT AEQ V (p: @pred AT AEQ (V * list V)), 
   crash_xform (crash_xform p) =p=> crash_xform p.
 Proof.
   unfold crash_xform, pimpl; intros.
@@ -697,7 +703,7 @@ Proof.
   eapply possible_crash_trans; eauto.
 Qed.
 
-Theorem crash_xform_idem_r : forall (p : rawpred),
+Theorem crash_xform_idem_r : forall AT AEQ V (p: @pred AT AEQ (V * list V)),
   crash_xform p =p=> crash_xform (crash_xform p).
 Proof.
   unfold crash_xform, pimpl, possible_crash; intros.
@@ -709,7 +715,7 @@ Proof.
   cbn; left; auto.
 Qed.
 
-Theorem crash_xform_idem : forall (p : rawpred),
+Theorem crash_xform_idem : forall AT AEQ V (p: @pred AT AEQ (V * list V)),
   crash_xform (crash_xform p) <=p=> crash_xform p.
 Proof.
   split.
@@ -717,7 +723,7 @@ Proof.
   apply crash_xform_idem_r.
 Qed.
 
-Theorem crash_xform_synced : forall p m,
+Theorem crash_xform_synced : forall AT AEQ V (p: @pred AT AEQ (V * list V)) m,
   crash_xform p m ->
   synced_mem m.
 Proof.
@@ -726,7 +732,7 @@ Proof.
   eapply possible_crash_synced; eauto.
 Qed.
 
-Theorem crash_xform_possible_crash_refl : forall p m,
+Theorem crash_xform_possible_crash_refl : forall AT AEQ V (p: @pred AT AEQ (V * list V)) m,
   crash_xform p m ->
   possible_crash m m.
 Proof.
@@ -748,13 +754,13 @@ Hint Rewrite crash_invariant_ptsto : crash_xform.
 
 Hint Resolve crash_invariant_emp.
 
-Lemma pred_apply_crash_xform : forall (p : rawpred) m m',
+Lemma pred_apply_crash_xform : forall AT AEQ V (p: @pred AT AEQ (V * list V)) m m',
   possible_crash m m' -> p m -> (crash_xform p) m'.
 Proof.
   unfold pimpl, crash_xform; eauto.
 Qed.
 
-Lemma pred_apply_crash_xform_pimpl : forall (p q : rawpred) m m',
+Lemma pred_apply_crash_xform_pimpl : forall AT AEQ V (p q: @pred AT AEQ (V * list V)) m m',
   possible_crash m m' -> p m -> crash_xform p =p=> q -> q m'.
 Proof.
   intros.
@@ -763,20 +769,18 @@ Proof.
 Qed.
 
 
-Definition possible_sync AT AEQ (m m' : @mem AT AEQ valuset) :=
+Definition possible_sync AT AEQ V (m m' : @mem AT AEQ (V * list V)) :=
   forall a, (m a = None /\ m' a = None) \/
   (exists v l l', m a = Some (v, l) /\ m' a = Some (v, l') /\ incl l' l).
 
-Theorem possible_sync_refl : forall AT AEQ (m: @mem AT AEQ _),
+Theorem possible_sync_refl : forall AT AEQ V (m: @mem AT AEQ (V * list V)),
     possible_sync m m.
 Proof.
   unfold possible_sync; intros.
   destruct (m a); intuition eauto 10 using incl_refl.
-  destruct v; right; intuition eauto.
-  repeat eexists; eauto using incl_refl.
 Qed.
 
-Theorem possible_sync_trans : forall AT AEQ (m1 m2 m3 : @mem AT AEQ _),
+Theorem possible_sync_trans : forall AT AEQ V (m1 m2 m3 : @mem AT AEQ (V * list V)),
   possible_sync m1 m2 ->
   possible_sync m2 m3 ->
   possible_sync m1 m3.
@@ -791,17 +795,17 @@ Proof.
   eapply incl_tran; eauto.
 Qed.
 
-Theorem possible_sync_sync_mem : forall AT AEQ (m : @mem AT AEQ valuset),
+Theorem possible_sync_sync_mem : forall AT AEQ V (m : @mem AT AEQ (V * list V)),
   possible_sync m (sync_mem m).
 Proof.
   unfold possible_sync, sync_mem; intros.
   destruct (m a); intuition.
-  right; destruct v.
+  right;
   repeat eexists.
   apply incl_nil.
 Qed.
 
-Theorem possible_sync_after_sync : forall A AEQ (m m': @mem A AEQ _),
+Theorem possible_sync_after_sync : forall A AEQ V (m m': @mem A AEQ (V * list V)),
     possible_sync (sync_mem m) m' ->
     m' = sync_mem m.
 Proof.
@@ -816,7 +820,7 @@ Proof.
   apply ListUtils.incl_in_nil in H2; subst; eauto.
 Qed.
 
-Theorem possible_sync_upd : forall AT AEQ (m : @mem AT AEQ _) a v l l',
+Theorem possible_sync_upd : forall AT AEQ V (m : @mem AT AEQ (V * list V)) a v l l',
   m a = Some (v, l) ->
   incl l' l ->
   possible_sync m (upd m a (v, l')).
@@ -839,12 +843,12 @@ Ltac xform' := autorewrite with crash_xform; repeat xform_simpl.
 Ltac xform := repeat xform'.
 
 
-Definition sync_invariant (p : rawpred) :=
+Definition sync_invariant {AT AEQ V} (p: @pred AT AEQ (V * list V)) :=
   (forall m m',
    possible_sync m m' ->
    p m -> p m').
 
-Theorem sync_xform_sync_invariant : forall p,
+Theorem sync_xform_sync_invariant : forall AT AEQ V (p: @pred AT AEQ (V * list V)),
   sync_invariant p ->
   sync_xform p =p=> p.
 Proof.
@@ -855,8 +859,8 @@ Proof.
 Qed.
 
 
-Theorem ptsto_pimpl_ptsto_subset : forall AT AEQ (a : AT) vs,
-  ((a |-> vs) : @pred AT AEQ _) =p=> a |+> vs.
+Theorem ptsto_pimpl_ptsto_subset : forall AT AEQ V (a : AT) vs,
+  ((a |-> vs) : @pred AT AEQ (V * list V)) =p=> a |+> vs.
 Proof.
   unfold pimpl, ptsto_subset; intros.
   exists (snd vs).
@@ -865,8 +869,8 @@ Proof.
   firstorder.
 Qed.
 
-Theorem ptsto_subset_pimpl_ptsto_ex : forall AT AEQ (a : AT) vs,
-  ((a |+> vs) : @pred AT AEQ _) =p=> a |->?.
+Theorem ptsto_subset_pimpl_ptsto_ex : forall AT AEQ V (a : AT) vs,
+  ((a |+> vs) : @pred AT AEQ (V * list V)) =p=> a |->?.
 Proof.
   unfold pimpl, ptsto_subset; intros.
   destruct H.
@@ -874,8 +878,8 @@ Proof.
   eexists; eauto.
 Qed.
 
-Theorem ptsto_subset_pimpl_ptsto : forall AT AEQ (a : AT) v,
-  ((a |+> (v, nil)) : @pred AT AEQ _) <=p=> a |=> v.
+Theorem ptsto_subset_pimpl_ptsto : forall AT AEQ V (a : AT) v,
+  ((a |+> (v, nil)) : @pred AT AEQ (V * list V)) <=p=> a |=> v.
 Proof.
   unfold ptsto_subset; intros; split.
   apply pimpl_exists_l; intros; simpl.
@@ -888,9 +892,9 @@ Proof.
   apply incl_nil.
 Qed.
 
-Theorem ptsto_subset_pimpl : forall AT AEQ (a : AT) v l l',
+Theorem ptsto_subset_pimpl : forall AT AEQ V (a : AT) v l l',
   incl l l' ->
-  ((a |+> (v, l)) : @pred AT AEQ _) =p=> a |+> (v, l').
+  ((a |+> (v, l)) : @pred AT AEQ (V * list V)) =p=> a |+> (v, l').
 Proof.
   unfold pimpl, ptsto_subset; intros.
   destruct H0.
@@ -899,8 +903,8 @@ Proof.
   eapply incl_tran; eauto.
 Qed.
 
-Theorem crash_xform_ptsto_subset' : forall a v,
-  crash_xform (a |+> v) =p=> exists v', [[ In v' (vsmerge v) ]] * a |+> (v', nil).
+Theorem crash_xform_ptsto_subset' : forall AT AEQ V a v,
+  @crash_xform AT AEQ V (a |+> v) =p=> exists v', [[ In v' (vsmerge v) ]] * a |+> (v', nil).
 Proof.
   intros; rewrite crash_xform_ptsto_subset.
   apply pimpl_exists_l; intros.
@@ -908,17 +912,17 @@ Proof.
   apply pimpl_exists_r; exists x; auto.
 Qed.
 
-Theorem ptsto_sync_mem : forall (a : addr) (vs : valuset) v m,
+Theorem ptsto_sync_mem : forall AT AEQ V a vs  v (m: @mem AT AEQ (V * list V)),
   (a |-> vs)%pred m ->
   v = fst vs ->
-  (a |-> (v, nil) : @pred _ addr_eq_dec _)%pred (sync_mem m).
+  (a |-> (v, nil))%pred (sync_mem m).
 Proof.
   unfold sync_mem, ptsto; destruct vs; intuition; subst.
   rewrite H1; simpl; auto.
   rewrite H2 by eauto; auto.
 Qed.
 
-Theorem possible_sync_ptsto : forall AT AEQ a v l (m m' : @mem AT AEQ _),
+Theorem possible_sync_ptsto : forall AT AEQ V a v l (m m' : @mem AT AEQ (V * list V)),
   possible_sync m m' ->
   (a |-> (v, l))%pred m ->
   (exists l', a |-> (v, l') * [[ incl l' l ]])%pred m'.
@@ -934,8 +938,8 @@ Proof.
 Qed.
 
 
-Theorem sync_invariant_ptsto_subset : forall a vs,
-  sync_invariant (a |+> vs)%pred.
+Theorem sync_invariant_ptsto_subset : forall AT AEQ V a vs,
+  @sync_invariant AT AEQ V (a |+> vs)%pred.
 Proof.
   unfold sync_invariant, pimpl, ptsto_subset, lift; intuition.
   destruct H0.
@@ -948,8 +952,8 @@ Proof.
   eapply incl_tran; eauto.
 Qed.
 
-Theorem sync_invariant_ptsto_any : forall a,
-  sync_invariant (a |->?)%pred.
+Theorem sync_invariant_ptsto_any : forall AT AEQ V a,
+  @sync_invariant AT AEQ V (a |->?)%pred.
 Proof.
   unfold sync_invariant, pimpl; intros.
   destruct H0; destruct x.
@@ -959,16 +963,16 @@ Proof.
   eexists; eauto.
 Qed.
 
-Theorem sync_xform_ptsto_subset_precise : forall a vs,
-  sync_xform (a |+> vs) =p=> a |=> (fst vs).
+Theorem sync_xform_ptsto_subset_precise : forall AT AEQ V a vs,
+  @sync_xform AT AEQ V (a |+> vs) =p=> a |=> (fst vs).
 Proof.
   unfold sync_xform, ptsto_subset, pimpl; intros.
   deex. destruct H0. apply sep_star_lift_apply in H; intuition.
   eapply ptsto_sync_mem; eauto.
 Qed.
 
-Theorem sync_xform_ptsto_subset_preserve : forall a vs,
-  sync_xform (a |+> vs) =p=> a |+> vs.
+Theorem sync_xform_ptsto_subset_preserve : forall AT AEQ V a vs,
+  @sync_xform AT AEQ V (a |+> vs) =p=> a |+> vs.
 Proof.
   intros.
   rewrite sync_xform_ptsto_subset_precise.
@@ -978,8 +982,8 @@ Proof.
   apply incl_nil.
 Qed.
 
-Theorem sync_invariant_ptsto_nil : forall a v,
-  sync_invariant (a |=> v)%pred.
+Theorem sync_invariant_ptsto_nil : forall AT AEQ V a v,
+  @sync_invariant AT AEQ V (a |=> v)%pred.
 Proof.
   unfold sync_invariant, pimpl; intros.
   eapply possible_sync_ptsto in H; [ | eauto ].
@@ -987,8 +991,8 @@ Proof.
   apply incl_in_nil in H2; subst; eauto.
 Qed.
 
-Theorem sync_invariant_emp :
-  sync_invariant emp.
+Theorem sync_invariant_emp : forall AT AEQ V,
+  @sync_invariant AT AEQ V emp.
 Proof.
   unfold sync_invariant, possible_sync, emp, pimpl; intros.
   specialize (H0 a).
@@ -997,20 +1001,20 @@ Proof.
   repeat deex. congruence.
 Qed.
 
-Theorem sync_xform_or_dist : forall p q,
+Theorem sync_xform_or_dist : forall AT AEQ V (p q: @pred AT AEQ (V * list V)),
   sync_xform (p \/ q) <=p=> sync_xform p \/ sync_xform q.
 Proof.
   firstorder.
 Qed.
 
-Theorem sync_xform_and_dist : forall p q,
+Theorem sync_xform_and_dist : forall AT AEQ V (p q: @pred AT AEQ (V * list V)),
   sync_xform (p /\ q) =p=> sync_xform p /\ sync_xform q.
 Proof.
   firstorder.
 Qed.
 
-Theorem sync_xform_lift_empty : forall (P : Prop),
-  @sync_xform [[ P ]] <=p=> [[ P ]].
+Theorem sync_xform_lift_empty : forall AT AEQ V (P : Prop),
+  @sync_xform AT AEQ V [[ P ]] <=p=> [[ P ]].
 Proof.
   unfold sync_xform, sync_mem, lift_empty, possible_crash; intros; split;
     intros m H; repeat deex.
@@ -1020,8 +1024,8 @@ Proof.
   rewrite H1; auto.
 Qed.
 
-Theorem sync_xform_emp :
-  sync_xform emp <=p=> emp.
+Theorem sync_xform_emp : forall AT AEQ V,
+  @sync_xform AT AEQ V emp <=p=> emp.
 Proof.
   unfold sync_xform, sync_mem, emp; split; intro; intros; repeat deex.
   destruct (m' a) eqn:?; congruence.
@@ -1030,16 +1034,16 @@ Proof.
   destruct (m x) eqn:?; congruence.
 Qed.
 
-Lemma sync_mem_union : forall AT AEQ (m1 m2 : @mem AT AEQ _),
+Lemma sync_mem_union : forall AT AEQ V (m1 m2 : @mem AT AEQ (V * list V)),
   sync_mem (mem_union m1 m2) = mem_union (sync_mem m1) (sync_mem m2).
 Proof.
   unfold mem_union, sync_mem; intros.
   apply functional_extensionality; intros.
   destruct (m1 x); auto.
-  destruct v; auto.
+  destruct p; auto.
 Qed.
 
-Lemma sync_mem_disjoint1 : forall AT AEQ (m1 m2 : @mem AT AEQ _),
+Lemma sync_mem_disjoint1 : forall AT AEQ V (m1 m2 : @mem AT AEQ (V * list V)),
   mem_disjoint m1 m2 -> mem_disjoint (sync_mem m1) (sync_mem m2).
 Proof.
   unfold mem_disjoint, sync_mem; intuition.
@@ -1051,7 +1055,7 @@ Proof.
   eauto.
 Qed.
 
-Lemma sync_mem_disjoint2 : forall AT AEQ (m1 m2 : @mem AT AEQ _),
+Lemma sync_mem_disjoint2 : forall AT AEQ V (m1 m2 : @mem AT AEQ (V * list V)),
   mem_disjoint (sync_mem m1) (sync_mem m2) -> mem_disjoint m1 m2.
 Proof.
   unfold mem_disjoint, sync_mem; intuition.
@@ -1065,7 +1069,7 @@ Hint Resolve sync_mem_disjoint1.
 Hint Resolve sync_mem_disjoint2.
 Hint Resolve sync_mem_union.
 
-Theorem sync_xform_sep_star_dist : forall (p q : rawpred),
+Theorem sync_xform_sep_star_dist : forall AT AEQ V (p q: @pred AT AEQ (V * list V)),
   sync_xform (p * q) <=p=> sync_xform p * sync_xform q.
 Proof.
   unfold_sep_star; unfold sync_xform, piff, pimpl; split; intros; repeat deex.
@@ -1074,21 +1078,21 @@ Proof.
     do 2 eexists; intuition.
 Qed.
 
-Theorem sync_xform_exists_comm : forall T (p : T -> rawpred),
+Theorem sync_xform_exists_comm : forall AT AEQ V T (p: T -> @pred AT AEQ (V * list V)),
   sync_xform (exists x, p x) <=p=> exists x, sync_xform (p x).
 Proof.
   split; unfold sync_xform, exis, pimpl; intros;
   repeat deex; repeat eexists; intuition eauto.
 Qed.
 
-Theorem sync_xform_forall_comm : forall T (p : T -> rawpred),
+Theorem sync_xform_forall_comm : forall AT AEQ V T (p: T -> @pred AT AEQ (V * list V)),
   sync_xform (foral x, p x) =p=> foral x, sync_xform (p x).
 Proof.
   unfold sync_xform, foral_, pimpl; intros.
   repeat deex; repeat eexists; intuition eauto.
 Qed.
 
-Theorem sync_xform_pimpl : forall p q,
+Theorem sync_xform_pimpl : forall AT AEQ V (p q: @pred AT AEQ (V * list V)),
   p =p=> q ->
   sync_xform p =p=> sync_xform q.
 Proof.
@@ -1096,53 +1100,54 @@ Proof.
   deex; eauto.
 Qed.
 
+
 Instance sync_xform_pimpl_proper:
-  Proper (pimpl ==> pimpl) sync_xform.
+  forall AT AEQ V, Proper (pimpl ==> pimpl) (@sync_xform AT AEQ V).
 Proof.
   firstorder.
 Qed.
 
 Instance sync_xform_flip_pimpl_proper:
-  Proper (Basics.flip pimpl ==> Basics.flip pimpl) sync_xform.
+  forall AT AEQ V, Proper (Basics.flip pimpl ==> Basics.flip pimpl) (@sync_xform AT AEQ V).
 Proof.
   firstorder.
 Qed.
 
 Instance sync_xform_piff_proper:
-  Proper (piff ==> piff) sync_xform.
+  forall AT AEQ V, Proper (piff ==> piff) (@sync_xform AT AEQ V).
 Proof.
   firstorder.
 Qed.
 
 Instance sync_invariant_piff_proper:
-  Proper (piff ==> Basics.impl) sync_invariant.
+  forall AT AEQ V, Proper (piff ==> Basics.impl) (@sync_invariant AT AEQ V).
 Proof.
   firstorder.
 Qed.
 
-Theorem sync_xform_diskIs: forall m,
+Theorem sync_xform_diskIs:  forall AT AEQ V (m: @mem AT AEQ (V * list V)),
   sync_xform (diskIs m) =p=> diskIs (sync_mem m).
 Proof.
   unfold sync_xform, diskIs, pimpl; intros.
   deex; auto.
 Qed.
 
-Theorem sync_xform_pred_apply : forall (p : rawpred) m,
+Theorem sync_xform_pred_apply :  forall AT AEQ V (p: @pred AT AEQ (V * list V)) m,
   p m -> (sync_xform p) (sync_mem m).
 Proof.
   firstorder.
 Qed.
 
-Theorem sync_mem_idem : forall AT AEQ (m : @mem AT AEQ _),
+Theorem sync_mem_idem : forall AT AEQ V (m : @mem AT AEQ (V * list V)),
   sync_mem (sync_mem m) = sync_mem m.
 Proof.
   unfold sync_mem; intros.
   apply functional_extensionality; intros.
   destruct (m x); auto.
-  destruct v; auto.
+  destruct p; auto.
 Qed.
 
-Theorem sync_xform_idem : forall p,
+Theorem sync_xform_idem :  forall AT AEQ V (p: @pred AT AEQ (V * list V)),
   sync_xform (sync_xform p) <=p=> sync_xform p.
 Proof.
   unfold sync_xform, piff, pimpl; split; intros; repeat deex.
@@ -1152,7 +1157,7 @@ Proof.
     rewrite sync_mem_idem; auto.
 Qed.
 
-Theorem sync_invariant_exists : forall T (p : T -> rawpred),
+Theorem sync_invariant_exists : forall AT AEQ V T (p: T -> @pred AT AEQ (V * list V)),
   (forall v, sync_invariant (p v)) ->
   sync_invariant (exists v, p v)%pred.
 Proof.
@@ -1160,7 +1165,7 @@ Proof.
   destruct H1. eexists. eauto.
 Qed.
 
-Theorem possible_sync_mem_union : forall AT AEQ (ma mb m' : @mem AT AEQ _),
+Theorem possible_sync_mem_union : forall AT AEQ V (ma mb m' : @mem AT AEQ (V * list V)),
   possible_sync (mem_union ma mb) m'
   -> @mem_disjoint _ _ _ ma mb
   -> exists ma' mb', m' = mem_union ma' mb' /\ mem_disjoint ma' mb' /\
@@ -1199,7 +1204,7 @@ Proof.
     congruence.
 Qed.
 
-Theorem possible_sync_disjoint : forall AT AEQ (ma mb ma' mb' : @mem AT AEQ _),
+Theorem possible_sync_disjoint : forall AT AEQ V (ma mb ma' mb' : @mem AT AEQ (V * list V)),
   @mem_disjoint _ _ _ ma' mb'
   -> possible_sync ma ma'
   -> possible_sync mb mb'
@@ -1214,7 +1219,8 @@ Proof.
   do 3 eexists; eauto.
 Qed.
 
-Theorem possible_sync_union : forall AT AEQ (ma mb ma' mb' : @mem AT AEQ _), possible_sync ma ma'
+Theorem possible_sync_union : forall AT AEQ V (ma mb ma' mb' : @mem AT AEQ (V * list V)),
+    possible_sync ma ma'
   -> possible_sync mb mb'
   -> possible_sync (mem_union ma mb) (mem_union ma' mb').
 Proof.
@@ -1235,7 +1241,7 @@ Proof.
 Qed.
 
 
-Theorem sync_invariant_sep_star : forall p q,
+Theorem sync_invariant_sep_star : forall AT AEQ V (p q: @pred AT AEQ (V * list V)),
   sync_invariant p ->
   sync_invariant q ->
   sync_invariant (p * q)%pred.
@@ -1245,8 +1251,8 @@ Proof.
   do 2 eexists. intuition eauto.
 Qed.
 
-Theorem sync_invariant_lift_empty : forall P,
-  sync_invariant [[ P ]]%pred.
+Theorem sync_invariant_lift_empty : forall AT AEQ V P,
+  @sync_invariant AT AEQ V [[ P ]]%pred.
 Proof.
   unfold sync_invariant; intros.
   apply star_emp_pimpl; apply pimpl_star_emp in H0.
@@ -1254,7 +1260,7 @@ Proof.
   eapply sync_invariant_emp; eauto.
 Qed.
 
-Theorem sync_invariant_and : forall p q,
+Theorem sync_invariant_and : forall AT AEQ V (p q: @pred AT AEQ (V * list V)),
   sync_invariant p ->
   sync_invariant q ->
   sync_invariant (p /\ q)%pred.
@@ -1262,7 +1268,7 @@ Proof.
   firstorder.
 Qed.
 
-Theorem sync_invariant_or : forall p q,
+Theorem sync_invariant_or : forall AT AEQ V (p q: @pred AT AEQ (V * list V)),
   sync_invariant p ->
   sync_invariant q ->
   sync_invariant (p \/ q)%pred.
@@ -1270,8 +1276,8 @@ Proof.
   firstorder.
 Qed.
 
-Lemma possible_sync_possible_crash_trans : forall m m1 m2,
-  possible_crash m m1 ->
+Lemma possible_sync_possible_crash_trans : forall AT AEQ V m m1 m2,
+  @possible_crash AT AEQ V m m1 ->
   possible_sync m1 m2 ->
   possible_crash m m2.
 Proof.
@@ -1284,7 +1290,7 @@ Proof.
   rewrite incl_in_nil with (l := l'); eauto.
 Qed.
 
-Lemma incl_vsmerge : forall l l' v,
+Lemma incl_vsmerge : forall V l l' (v: V),
     incl l l' ->
     incl (vsmerge (v, l)) (vsmerge (v, l')).
 Proof.
@@ -1297,8 +1303,8 @@ Proof.
     specialize (H a0); simpl in *; intuition eauto.
 Qed.
 
-Lemma possible_crash_possible_sync_trans : forall m m1 m2,
-    possible_sync m m1 ->
+Lemma possible_crash_possible_sync_trans : forall AT AEQ V m m1 m2,
+    @possible_sync AT AEQ V m m1 ->
     possible_crash m1 m2 ->
     possible_crash m m2.
 Proof.
@@ -1310,7 +1316,7 @@ Proof.
   eapply incl_vsmerge; eauto.
 Qed.
 
-Theorem sync_invariant_crash_xform : forall F,
+Theorem sync_invariant_crash_xform : forall AT AEQ V (F: @pred AT AEQ (V * list V)),
   sync_invariant (crash_xform F).
 Proof.
   unfold sync_invariant, crash_xform; intros; deex.
@@ -1341,7 +1347,7 @@ Qed.
 
 Hint Resolve sync_invariant_mem_pred.
 *)
-Theorem upd_sync_invariant : forall (p : @pred _ _ _) m a v l l',
+Theorem upd_sync_invariant : forall AT AEQ V (p: @pred AT AEQ (V * list V)) m a v l l',
   sync_invariant p ->
   p m ->
   m a = Some (v, l) ->
@@ -1353,7 +1359,7 @@ Proof.
   eapply possible_sync_upd; eauto.
 Qed.
 
-Theorem ptsto_subset_valid : forall AT AEQ a vs F (m : @mem AT AEQ _),
+Theorem ptsto_subset_valid : forall AT AEQ V a vs F (m : @mem AT AEQ (V * list V)),
   (a |+> vs * F)%pred m ->
   exists l, m a = Some (fst vs, l) /\ incl l (snd vs).
 Proof.
@@ -1366,7 +1372,7 @@ Proof.
   apply H5.
 Qed.
 
-Theorem ptsto_subset_valid' : forall AT AEQ a vs F (m : @mem AT AEQ _),
+Theorem ptsto_subset_valid' : forall AT AEQ V a vs F (m : @mem AT AEQ (V * list V)),
   (F * a |+> vs)%pred m ->
   exists l, m a = Some (fst vs, l) /\ incl l (snd vs).
 Proof.
@@ -1375,7 +1381,7 @@ Proof.
   eapply ptsto_subset_valid; eauto.
 Qed.
 
-Lemma ptsto_subset_upd : forall v0 v a m vs vs' vs0 (F : rawpred),
+Lemma ptsto_subset_upd : forall AT AEQ V (F: @pred AT AEQ (V * list V)) v0 v a m vs vs' vs0,
   (F * a |+> (v0, vs0))%pred m ->
   incl vs' vs ->
   (F * a |+> (v, vs))%pred (upd m a (v, vs')).
@@ -1400,7 +1406,7 @@ Qed.
 
 
 Lemma sync_invariant_sync_mem_apply:
-  forall (P: rawpred) m,
+ forall AT AEQ V (P: @pred AT AEQ (V * list V)) m,
     P m ->
     sync_invariant P ->
     P (sync_mem m).
